eliminate domain

map-union.dfy
@@ -1,8 +1,3 @@
-function domain(m:map<int, int>) : set<int>
-{
-    set k | k in m
-}
-
 lemma disjointness_lemma(a:set<int>, b:set<int>)
     requires a * b == {};
     ensures forall k :: k in a + b && k in b ==> !(k in a);
@@ -18,12 +13,12 @@ lemma disjointness_lemma(a:set<int>, b:set<int>)
 }
 
 function mapunion(a:map<int, int>, b:map<int, int>) : map<int, int>
-    requires domain(a) * domain(b) == {};
-    ensures domain(a) + domain(b) == domain(mapunion(a, b));
-    ensures forall k :: k in domain(a) ==> a[k] == mapunion(a,b)[k];
-    ensures forall k :: k in domain(b) ==> b[k] == mapunion(a,b)[k];
+    requires a.Keys * b.Keys == {};
+    ensures a.Keys + b.Keys == mapunion(a, b).Keys;
+    ensures forall k :: k in a.Keys ==> a[k] == mapunion(a,b)[k];
+    ensures forall k :: k in b.Keys ==> b[k] == mapunion(a,b)[k];
 {
-    var c := map k| k in domain(a) + domain(b) :: if k in domain(a) then a[k] else b[k];
-    disjointness_lemma(domain(a), domain(b));
+    var c := map k| k in a.Keys + b.Keys :: if k in a.Keys then a[k] else b[k];
+    disjointness_lemma(a.Keys, b.Keys);
     c
 }
